# Haskell Programing from First Principal

## Chap 1 - All you need is Lambda. 

- The lambda in lambda calculus is the greek letter ðœ† used to introduce, or abstract, arguments for binding in an expression.
- A lambda abstraction is an anonymous function or lambda term.
(ðœ†ð‘¥.ð‘¥ + 1)
The head of the expression, ðœ†ð‘¥., abstracts out the term ð‘¥ + 1. We can apply it to any ð‘¥ and recompute different results for each ð‘¥ to which we apply the lambda.

## Chap 2 - Hello Haskell.
- argument vs parameter
- An expression is a combination of symbols that conforms to syntactic rules and can be evaluated to some result.
- A value is an expression that cannot be reduced or evalu- ated any further. 
- A function is a mathematical object that can be applied to an argument in order to return a result
- Syntactic sugar is syntax within a programming language designed to make expressions easier to read and write

## Chap 3 - Strings
- String is represented by a linked list of Char values, aka [Char]
- A type or datatype is a classification of values or data.
- Concatenation is the joining together of sequences of val- ues.
  ```
  Prelude> "tacos" ++ " " ++ "rock"
     "tacos rock"
  ```

- scope is where a variable can be validly referred to by name in a program

## Chap 4 - Datatypes
- A tuple is an ordered grouping of values.
  - unit or () : zero tuple
- A type class is a set of operations defined with respect to a polymorphic type.
- Data constructors in Haskell provide a means of creating values that inhabit a given type.
  - data Pet = Cat | Dog Name
- Type constructors in Haskell are not values and can only be used in type signatures.
- Data declarations define new datatypes in Haskell. Data declarations always create a new type constructor but may or may not create new data constructors. Data declarations are how we refer to the entire definition that begins with the data keyword.
- A type alias is a way to refer to a type constructor or type constant by an alternate name, usually to communicate something more specific or for brevity:
  ``` 
  type Name = String
  ```
- Polymorphism in Haskell, specifically, is either parametric or constrained. 
- Parametric or ad-hoc polymorphic function:
  ```
  id :: a -> a
  id x = x

- Constrained or Boundedv Polymorphic
  ```
  isEqual :: Eq a => a -> a -> Bool 
  isEqual x y = x == y

## Chap 5 - Types
- Type inference is to infer principal types(most generic type that still type checks) from terms without requiring explicit type annotations.
- A type variable is a way to refer to an unspecified type or set of types in Haskell type signatures.
- A type class is a means of expressing faculties or interfaces that multiple datatypes may have in common. 
- Parametricity is the property that holds in the presence of parametric polymorphism. 
- A module is the unit of organization that the Haskell pro- gramming language uses to collect together declarations of values, functions, datatypes, type classes, and type class instances.

## Chap 6 - Type Classes
- Type class inheritance is when a type class has a superclass. This is a way of expressing that a type class requires another type class to be available for a given type before you can write an instance:
  ```
  class Num a => Fractional a where 
    (/) :: a -> a -> a
    recip :: a -> a
    fromRational :: Rational -> a

- IO is the type for values whose evaluation bears the possi- bility of causing side effects, such as printing text, reading text input from the user, reading or writing to files, or connecting to remote computers. 
- An instance is the definition of how a type class should work for a given type.

See [Practice](../practice/typeCheck) for Chap 6 & 7

## Chap 7 - More Functional Patterns
- anonymous function
  ```
  triple x = x * 3
  (\x -> x * 3)

  with specific type
  (\x -> x * 3) :: Integer -> Integer
  (\x -> x * 3 :: Integer)

  ghci> (\x -> x * 3) 1

  mTh x y z = x * y * z
  mTh x y = \z -> x * y * z
  mTh x = \y -> \z -> x * y * z
  mTh = \x -> \y -> \z -> x * y * z

  ```
  
- pattern matching
  ```
  isItTwo :: Integer -> Bool
  isItTwo 2 = True
  isItTwo _ = False

  f :: (a, b) -> (c, d) -> ((b, d), (a, c)) 
  f x y = ((snd x, snd y), (fst x, fst y))
  f (a, b) (c, d) = ((b, d), (a, c))

  fst3 :: (a, b, c) -> a
  fst3 (x, _, _) = x

  returnLast :: a -> b -> c -> d -> d 
  returnLast _ _ _ d = d

  ```
- case expressions
  ```
  funcZ x =
    case x + 1 == 1 of
      True -> "AWESOME" 
      False -> "wut"
  ```

- HOF
  ```
  myf :: (a -> b) -> a -> c -> b
  myf f a c = f a
  ```

  Exercise: Artful dodgy - [sol](./ch7/artfulDodgy.hs)

- Guards
  ```
  myAbs :: Integer -> Integer 
  myAbs x
    | x < 0 = (-x) 
    | otherwise = x

  dogYrs :: Integer -> Integer 
  dogYrs x
    | x<=0 =0
    | x<=1 = x * 15
    | x<=2 = x * 12
    | x<=4 = x * 8
    | otherwise = x * 6
  ```

  Exercise: Guard Duty - [sol](./ch7/guardDuty.hs)

- Function composition
  ```
  f g x
  (f.g) x
  f (g x)
  f.g $ x

  negate sum xs
  negate . sum $ xs
  (negate . sum) xs

  take 5 . enumFrom $ 3

  take 5 . filter odd . enumFrom $ 3 

  ```

- Point-free style
  composing functions without parameter
  ``` 
  (f . g) x = f (g x)
  f . g = \x -> f (g x)
  f . g . h = \x -> f (g (h x))

  ```
  [arith2.hs](./ch7/arith2.hs)

## Chap 8 - Recursion
  ```
  factorial :: Integer -> Integer 
  factorial 0 = 1
  factorial n = n * factorial (n - 1)

  fibonacci :: Integral a => a -> a 
  fibonacci 0 = 0
  fibonacci 1 = 1
  fibonacci x = fibonacci (x - 1) + fibonacci (x - 2)
  ```
## Chap 9 - List
  WHNF(Weak Head Normal Form) - the expression is only evaluated as far as is necessary to reach a data constructor or lamda.
    top most thing outer most thing is top most constructor
    top most thing lamda

  NF(Normal Form) - the expression is fully evaluated.
  ```
  (1, 2) -- WHNF & NF
  (1, 1 + 1) -- WHNF & not NF
  \x -> x * 10 -- WHNF & NF
  "Papu" ++ "chon" -- not WHNF & not NF
  num :: [Int]; num = [1,2,3] -- WHNF & not NF (Note: `[1,2,3]` gets compiled to `1:(_{2:3:[]}_)`)
  num :: [Int]; myNum = [1..10] â€“ not WHNF & not NF  (Note: `[1..10]` gets compiled to `enumFromTo 1 10`)
  
  [1,2,3,4,5] -- WHNF & NF (good!) 
  1:2:3:4:_ -- WHNF & not NF (good!)
  enumFromTo 1 10 -- not WHNF & not NF (good!)
  length [1,2,3,4,5] -- not WHNF & NF (to be NF, it must first be WHNF.)
  sum (enumFromTo 1 10) -- not WHNF & not NF (good!)
  ['a'..'m'] ++ ['n'..'z'] -- not WHNF & not NF (good!)
  (_, 'b') -- WHNF & not NF (good! the root of the syntax tree is a data constructor)


  f(x) = x^2 - 2x - 4

  g(x) = 1 - x^3

  h(x) = (3x + f(1 - 3x)) / g(x - 4)


  suppose we need h(4)

  traditionally, we start on the inner most pieces, the leaves of the syntax tree.
  h(4) = (3*4 + f(1-3*4))/g(4-4)
       = (12 + f(1-12))/g(0)
       = (12 + f(-11))/(1 - 0^3)
       = (12 + ((-11)^2 - 2*(-11) - 4)) / (1 - 0)

  but what if i told you that we don't have to start on the inside first? (morpheus look)
  h(x) = (3x + f(1 - 3x)) / g(x - 4)
  h(x) = (3x + ( (1-3x)^2 - 2*(1-3x) - 4) / (1 - (x - 4)^3)
                 ^ we evaluated f without evaluating its argument first!
                            ^ same, evaluated g before evaluating its arg!



  ```

  strict evaluation is when you evaluate your arguments before evaluating the function.
  This is how C, Java, Javascript, Python almost every programming language works.

  lazy evaluation is when you evaluate your functions before evaluating their arguments.
  This is how (most things in) Haskell (usually) works.

  Haskell is not necessarily lazy. Compiler chooses strictness according to the categories in Strictness analyzer.

## Chap 10 - Folding Lists
  Fold is a HOF that given a function to accumulate the results and returns the built up value.

  ```
  foldr :: Foldable t => (a -> b -> b) -> b -> t a -> b
  foldl :: Foldable t => (b -> a -> b) -> b -> t a -> b
  ```

  A catamorphism is a generalization of folds to arbitrary datatypes. Where a fold allows you to break down a list into an arbitrary
datatype, a catamorphism is a means of breaking down the structure of any datatype.

  ```
  data Bool = False | True
  bool :: a -> a -> Bool -> a
  ```

  ```
  foldr f z [] = z
  foldr f z (x:xs) = f x (foldr f z xs)

  foldl f z [] = z
  foldl f z (x:xs) = foldl f (f z x) xs
  ```

## Chap 11 - Folding Lists



